imp2asm made, yet to be proved

imp_compile/test.ml
@@ -38,12 +38,41 @@ open ImpLink
  *   List.fold_left add_builtin p C2C.builtins_generic.builtin_functions *)
 
 
-let convert_builtin (name, (out, ins, b)) =
+(* let convert_builtin (name, (out, ins, b)) =
+ *   let env = Env.empty in
+ *   let id = Camlcoq.intern_string name in
+ *   let id' = Camlcoq.coqstring_of_camlstring name in
+ *   let targs = List.map (C2C.convertTyp env) ins
+ *                 |> Imp2Asm.ASMGEN.list_type_to_typelist in
+ *   let tres = C2C.convertTyp env out in
+ *   let sg = Ctypes.signature_of_type targs tres AST.cc_default in
+ *   let ef =
+ *     if name = "malloc" then AST.EF_malloc else
+ *     if name = "free" then AST.EF_free else
+ *     if Str.string_match C2C.re_runtime name 0 then AST.EF_runtime(id', sg) else
+ *     if Str.string_match C2C.re_builtin name 0
+ *     && List.mem_assoc name C2C.builtins.builtin_functions
+ *     then AST.EF_builtin(id', sg)
+ *     else AST.EF_external(id', sg) in
+ *   let decl = (id, AST.Gfun (AST.External ef)) in
+ *   decl *)
+
+(* let malloc_dec =
+ *   ("malloc", (TPtr(TVoid [], []), [TPtr(TVoid [], [])], false))
+ * 
+ * let free_dec =
+ *   ("free", (TVoid [], [TPtr(TVoid [], [])], false)) *)
+
+(* let app_builtins p =
+ *   { p with AST.prog_defs = builtins @ p.AST.prog_defs } *)
+
+
+
+let get_builtin (name, (out, ins, b)) =
   let env = Env.empty in
-  let id = Camlcoq.intern_string name in
   let id' = Camlcoq.coqstring_of_camlstring name in
   let targs = List.map (C2C.convertTyp env) ins
-                |> Imp2Asm.ASMGEN.list_type_to_typelist in
+                |> Imp2Asm.list_type_to_typelist in
   let tres = C2C.convertTyp env out in
   let sg = Ctypes.signature_of_type targs tres AST.cc_default in
   let ef =
@@ -54,46 +83,54 @@ let convert_builtin (name, (out, ins, b)) =
     && List.mem_assoc name C2C.builtins.builtin_functions
     then AST.EF_builtin(id', sg)
     else AST.EF_external(id', sg) in
-  let decl = (id, AST.Gfun (AST.External ef)) in
+  let decl = (id', AST.Gfun (AST.External ef)) in
   decl
 
-let malloc_dec =
-  ("malloc", (TPtr(TVoid [], []), [TPtr(TVoid [], [])], false))
-
-let free_dec =
-  ("free", (TVoid [], [TPtr(TVoid [], [])], false))
-
 let builtins =
-  List.map convert_builtin (C2C.builtins_generic.builtin_functions @ [malloc_dec; free_dec])
-
-let app_builtins p =
-  { p with AST.prog_defs = builtins @ p.AST.prog_defs }
+  List.map get_builtin C2C.builtins_generic.builtin_functions
 
 
 (* Csharpminor program compilation *)
-let compile_csm p ofile =
-  let cl_built = app_builtins p in
-  (* Convert to Asm *)
-  (match Compiler.apply_partial
-           (Imp2Asm.ASMGEN.transf_csharpminor_program cl_built)
-           Asmexpand.expand_program with
-   | Errors.OK asm ->
-      (* Print Asm in text form *)
-      let oc = open_out ofile in
-      PrintAsm.print_program oc asm;
-      close_out oc
-   | Errors.Error msg ->
-      let loc = file_loc ofile in
-      fatal_error loc "%a"  print_error msg)
+(* let compile_csm p ofile =
+ *   let cl_built = app_builtins p in
+ *   (\* Convert to Asm *\)
+ *   (match Compiler.apply_partial
+ *            (Imp2Asm.ASMGEN.transf_csharpminor_program cl_built)
+ *            Asmexpand.expand_program with
+ *    | Errors.OK asm ->
+ *       (\* Print Asm in text form *\)
+ *       let oc = open_out ofile in
+ *       PrintAsm.print_program oc asm;
+ *       close_out oc
+ *    | Errors.Error msg ->
+ *       let loc = file_loc ofile in
+ *       fatal_error loc "%a"  print_error msg) *)
 
+
+(* (\* Imp program compilations *\)
+ * let compile_imp p ofile =
+ *   (\* Convert Imp to Csharpminor *\)
+ *   let i2c = Imp2Csharpminor.compile_imp p in
+ *   match i2c with
+ *   | Errors.OK csm_out ->
+ *      compile_csm csm_out ofile
+ *   | Errors.Error msg ->
+ *      let loc = file_loc ofile in
+ *      fatal_error loc "%a"  print_error msg *)
 
 (* Imp program compilations *)
 let compile_imp p ofile =
-  (* Convert Imp to Csharpminor *)
-  let i2c = Imp2Csharpminor.compile_imp p in
-  match i2c with
-  | Errors.OK csm_out ->
-     compile_csm csm_out ofile
+  (* Convert Imp to Asm *)
+  let i2a =
+    (Compiler.apply_partial
+       (Imp2Asm.compile_imp builtins p)
+       Asmexpand.expand_program) in
+  match i2a with
+  | Errors.OK asm ->
+     (* Print Asm in text form *)
+     let oc = open_out ofile in
+     PrintAsm.print_program oc asm;
+     close_out oc
   | Errors.Error msg ->
      let loc = file_loc ofile in
      fatal_error loc "%a"  print_error msg
@@ -102,10 +139,16 @@ let compile_imp p ofile =
 (* Imp programL compilations for linked imps *)
 let compile_impL p ofile =
   (* Convert Imp to Csharpminor *)
-  let i2c = Imp2Csharpminor.compile p in
-  match i2c with
-  | Errors.OK csm_out ->
-     compile_csm csm_out ofile
+  let i2a =
+    (Compiler.apply_partial
+       (Imp2Asm.compile builtins p)
+       Asmexpand.expand_program) in
+  match i2a with
+  | Errors.OK asm ->
+     (* Print Asm in text form *)
+     let oc = open_out ofile in
+     PrintAsm.print_program oc asm;
+     close_out oc
   | Errors.Error msg ->
      let loc = file_loc ofile in
      fatal_error loc "%a"  print_error msg
@@ -123,7 +166,9 @@ let main =
   compile_imp (ImpMem1.imp_mem1_f) "mem1F.s";
   compile_imp (ImpMem1.imp_mem1_main) "mem1Main.s";
   compile_imp (ImpMem2.imp_mem2_prog) "mem2.s";
-  let _link1 = (Imp2CsharpminorLink.link_imps [ImpLink.imp_linkMain_prog; ImpLink.imp_linkF_prog; ImpLink.imp_linkG_prog]) in
+  let _link1 =
+    (Imp2Csharpminor.link_imps builtins
+       [ImpLink.imp_linkMain_prog; ImpLink.imp_linkF_prog; ImpLink.imp_linkG_prog]) in
   match _link1 with
   | Some link1 ->
      print_endline "link1 succeed.";
