imp/Imp2Asm.v
@@ -1,12 +1,13 @@
 Require Import Coqlib.
 Require Import Universe.
+Require Import Imp.
 Require Import Imp2Csharpminor.
 
 From compcert Require Import Ctypes Errors Compiler.
 
 Set Implicit Arguments.
 
-Module ASMGEN.
+Section ASMGEN.
 
   (* For builtins at compile time, ref: Velus, Generation.v *)
   Fixpoint list_type_to_typelist (types: list type): typelist :=
@@ -20,5 +21,15 @@ Module ASMGEN.
     OK p
        @@@ time "Cminor generation" Cminorgen.transl_program
        @@@ transf_cminor_program.
+
+  Context `{builtins: builtinsTy}.
+
+  Definition compile (src: Imp.programL) : res Asm.program :=
+    match Imp2Csharpminor.compile src with
+    | OK csm => transf_csharpminor_program csm
+    | Error msg => Error msg
+    end.
+
+  Definition compile_imp (src: Imp.program) := compile (Imp.lift src).
 
 End ASMGEN.
