imp/Imp2CsharpminorMatch.v
@@ -113,12 +113,14 @@ Section MATCH.
   Definition imp_stack := (r_state * p_state * (lenv * val)) -> imp_state.
 
   (* Hypothesis archi_ptr64 : Archi.ptr64 = true. *)
+  Context `{builtins : builtinsTy}.
+
   Definition ext_len : Imp.programL -> nat := fun src => List.length (src.(ext_varsL)) + List.length (src.(ext_funsL)).
   Definition int_len : Imp.programL -> nat := fun src => List.length src.(defsL).
   (* next block of src's initialized genv *)
   Definition src_init_nb : Imp.programL -> nat := fun src => int_len src.
   (* next block of tgt's initialized genv *)
-  Definition tgt_init_len := List.length (init_g ++ c_sys).
+  Definition tgt_init_len := List.length ((@init_g builtins) ++ c_sys).
   Definition tgt_init_nb : Imp.programL -> Values.block := fun src => Pos.of_succ_nat (tgt_init_len + (ext_len src) + (int_len src)).
 
   Definition get_sge (src : Imp.programL) := Sk.load_skenv (Sk.sort (ImpMod.get_modL src).(ModL.sk)).
